reflex case stadies/TrafficLights/trafficLights_VC10.thy
@@ -1,0 +1,124 @@
+theory trafficLights_VC10
+imports trafficLightsTheory
+begin
+
+lemma extra:
+ assumes base_inv:"(extraInv st0)"
+ and st1:"(st1=(setVarBool st0 ''button'' button))"
+ and st1_Controller_state:"(getPstate st1 ''Controller'')=''green''"
+ and st1_green_timeout:"30000>(ltime st1 ''Controller'')"
+ and st2:"(st2=(toEnv st1))"
+ and st_final:"(st_final=st2)"
+shows "(extraInv st_final)"
+  by sorry
+
+
+lemma
+ assumes base_inv:"(inv2 st0)"
+ and st1:"(st1=(setVarBool st0 ''button'' button))"
+ and st1_Controller_state:"(getPstate st1 ''Controller'')=''green''"
+ and st1_green_timeout:"30000>(ltime st1 ''Controller'')"
+ and st2:"(st2=(toEnv st1))"
+ and st_final:"(st_final=st2)"
+shows "(inv2 st_final)"
+proof(simp only:inv2_def;rule conjI)
+  show "extraInv st_final" using assms extra inv2_def by auto
+next
+  have extra:"extraInv st_final \<and> extraInv st0 \<and> R2 st0" using assms extra inv2_def by auto
+  show "R2 st_final"
+  proof -
+    have 0:"toEnvP st0 \<and> toEnvP st_final \<and> st0 = predEnv st_final" using assms inv2_def extraInv_def by auto
+    moreover have "P3_cons R2_A st0" using assms inv2_def R2_to_P3_cons by auto
+    moreover have "(p_2_3_conpred R2_A st_final) st_final"
+      apply (simp only: p_2_3_conpred_def R2_A_def)
+      by blast
+    moreover have "P1 (p_2_3_conpred R2_A st_final) st0"
+    proof (simp only: P1_def p_2_3_conpred_def R2_A_def SMT.verit_bool_simplify(4);rule allI;rule impI)
+      show "getVarBool st_final ''light'' = True" using assms extra extraInv_def extra3_def substate_refl by auto
+    qed
+    ultimately have "P3_cons R2_A st_final" using P3_lemma by auto
+    thus ?thesis using P3_cons_to_R2 assms by auto
+  qed
+qed
+
+lemma
+ assumes base_inv:"(inv5 st0)"
+ and st1:"(st1=(setVarBool st0 ''button'' button))"
+ and st1_Controller_state:"(getPstate st1 ''Controller'')=''green''"
+ and st1_green_timeout:"30000>(ltime st1 ''Controller'')"
+ and st2:"(st2=(toEnv st1))"
+ and st_final:"(st_final=st2)"
+shows "(inv5 st_final)"
+proof(simp only:inv5_def;rule conjI)
+  show "extraInv st_final" using assms extra inv5_def by auto
+next
+  have extra1:"extraInv st0 \<and> R5 st0" using assms inv5_def by auto
+  have extra2:"extraInv st_final" using assms extra inv5_def by auto
+  show "R5 st_final"
+  proof -
+    have 0:"toEnvP st0 \<and> toEnvP st_final \<and> st0 = predEnv st_final" using assms inv5_def extraInv_def by auto
+    moreover have "P3_cons R5_A st0" using assms inv5_def R5_to_P3_cons by auto
+    moreover have "(p_2_3_conpred R5_A st_final) st_final"
+      apply (simp only: p_2_3_conpred_def R5_A_def)
+      by blast
+    moreover have "P1 (p_2_3_conpred R5_A st_final) st0"
+    proof (simp only: P1_def p_2_3_conpred_def R5_A_def SMT.verit_bool_simplify(4);rule allI;rule impI)
+      fix x
+      assume prem:"(toEnvP x \<and> substate x st0) \<and>
+               toEnvNum x st_final < 150 \<and>
+               getVarBool (predEnv x) ''light'' \<noteq> False \<and>
+               getVarBool x ''light'' = False"
+      have 1:"toEnvNum x st0 < 149" using 0 prem predEnv_substate predEnv_toEnvNum toEnvNum3 by force
+      have 2:"toEnvP (predEnv x)" using prem predEnvP_or_emptyState by force
+      have 3:"substate (predEnv x) st0" using predEnv_substate prem substate_trans by blast
+      have 4:"getPstate (predEnv x) ''Controller'' = ''green''" using prem 2 3  extra1 extraInv_def extra0_def extra4_def by auto
+      have a4:"getPstate x ''Controller'' \<noteq> ''green''" using prem extra1 extraInv_def extra0_def extra3_def by auto
+      have 5:"(ltime st0 ''Controller'') div 100 <300" using assms by auto
+      have 6:"toEnvNum (predEnv x) st0 <150" using 1 predEnv_substate predEnv_toEnvNum prem toEnvNum3 by force
+      consider (a)"toEnvNum x st0 < (ltime st0 ''Controller'') div 100" | (b)"toEnvNum x st0 \<ge> (ltime st0 ''Controller'') div 100" by force
+      thus "getVarBool st_final ''light'' = False"
+      proof(cases)
+        case a
+        moreover have "toEnvP x \<and> toEnvP st0 \<and> substate x st0 \<and> substate st0 st0" using 0 prem substate_refl by auto
+        moreover have "getPstate st0 ''Controller'' = ''green''" using assms by auto
+        ultimately have "getPstate x ''Controller'' = ''green'' " using extra1 extraInv_def extra13_def by blast
+        then have "getVarBool x ''light''" using prem extra1 extraInv_def extra3_def by auto
+        then show ?thesis using prem by auto
+      next
+        case b
+        then have 7:"toEnvNum (predEnv x) st0 > (ltime st0 ''Controller'') div 100" using toEnvNum3 predEnv_substate predEnv_toEnvNum prem by force
+        have "getPstate st0 ''Controller''= ''green''" using assms by auto
+        then obtain y where o1:"toEnvP y \<and> substate y st0 \<and>
+                                toEnvNum y st0 = ltime st0 ''Controller'' div 100\<and>
+                                getPstate y ''Controller'' = ''redToGreen'' \<and>
+                                ltime y ''Controller'' \<ge> 5000" 
+          using extra1 extraInv_def extra12_def 0 substate_refl by blast
+        then have "substate (predEnv x) y \<or> substate y (predEnv x)" using substate_total 3 by auto
+        then consider (c) "substate (predEnv x) y" | (d) "substate y (predEnv x) \<and> (predEnv x)\<noteq>y" by auto
+        then show "getVarBool st_final ''light'' = False"
+        proof (cases)
+          case c
+          then have "toEnvNum (predEnv x) st0 = toEnvNum (predEnv x) y + toEnvNum y st0" using o1 toEnvNum3 by auto
+          then have 8:"toEnvNum (predEnv x) y < 150" using 6 by auto
+          have "ltime y ''Controller'' div 100 \<ge> 50" using o1 by auto
+          then have "100 + 1 + (ltime y ''Controller'' div 100) \<ge> 150" by auto
+          then have "toEnvP (predEnv x) \<and> toEnvP y \<and> 
+                      substate (predEnv x) y \<and> substate y st0 \<and>
+                      getPstate y ''Controller'' = ''redToGreen'' \<and>
+                      toEnvNum (predEnv x) y \<le> 100 + 1 + (ltime y ''Controller'' div 100)" using 2 o1 c 3 8 by auto
+          then have "getVarBool (predEnv x) ''light'' = False" using extra1 extraInv_def extra18_def by auto
+          then show ?thesis using prem by auto
+        next
+          case d
+          then have "toEnvNum y st0 = toEnvNum y (predEnv x) + toEnvNum (predEnv x) st0" using 3 toEnvNum3 by auto
+          then have "ltime st0 ''Controller'' div 100 = toEnvNum y (predEnv x) + toEnvNum (predEnv x) st0" using o1 by auto
+          then show ?thesis using 7 by auto 
+        qed
+      qed
+    qed
+    ultimately have "P3_cons R5_A st_final" using P3_lemma by auto
+    thus ?thesis using P3_cons_to_R5 assms by auto
+  qed
+qed
+
+end
